\documentclass{article}%
\usepackage[T1]{fontenc}%
\usepackage[utf8]{inputenc}%
\usepackage{lmodern}%
\usepackage{textcomp}%
\usepackage{lastpage}%
\usepackage{geometry}%
\geometry{head=2.5cm,left=3cm,right=3cm,bottom=2.5cm}%
\usepackage{ragged2e}%
\usepackage{amsmath}%
%
%
%
\begin{document}%
\normalsize%
\begin{center}%
\section*{}%
\label{sec:}%
\begin{Large}%
\textbf{Generalized S{-}I{-}R model}%
\end{Large}

%
\end{center}%
\section{Equations}%
\label{sec:Equations}%
\begin{large}%
These are the equations for the model:%
\end{large}

%
\begin{alignat*}{2}%
\frac{dE_{1}}{dt} &= \Theta_{1}E_{1} +  \mu_{1}R_{1} +  \Lambda_{1}R_{1} +  \delta_{1} -  \Lambda_{1}R_{1} -  \delta_{1} \\ &%
\end{alignat*}%
\begin{alignat*}{2}%
\frac{dE_{2}}{dt} &= \Theta_{2}E_{2} +  \mu_{2}R_{2} +  \Lambda_{2}R_{2} +  \delta_{2} -  \Lambda_{2}R_{2} -  \delta_{2} \\ &%
\end{alignat*}%
\begin{alignat*}{2}%
\frac{dE_{3}}{dt} &= \Theta_{3}E_{3} +  \mu_{3}R_{3} +  \Lambda_{3}R_{3} +  \delta_{3} -  \Lambda_{3}R_{3} -  \delta_{3} \\ &%
\end{alignat*}%
\begin{alignat*}{2}%
\frac{dI\_pre_{1}}{dt} &= \Theta_{1}I\_{pre}_{1} +  \mu_{1}E_{1} +%
\end{alignat*}%
\begin{alignat*}{2}%
\frac{dI\_pre_{2}}{dt} &= \Theta_{2}I\_{pre}_{2} +  \mu_{2}E_{2} +%
\end{alignat*}%
\begin{alignat*}{2}%
\frac{dI\_pre_{3}}{dt} &= \Theta_{3}I\_{pre}_{3} +  \mu_{3}E_{3} +%
\end{alignat*}%
\begin{alignat*}{2}%
\frac{dI\_symp\_s_{1}}{dt} &= \Theta_{1}I\_{symp}\_{s}_{1} +  \mu_{1}I\_{pre}_{1} +%
\end{alignat*}%
\begin{alignat*}{2}%
\frac{dI\_symp\_s_{2}}{dt} &= \Theta_{2}I\_{symp}\_{s}_{2} +  \mu_{2}I\_{pre}_{2} +%
\end{alignat*}%
\begin{alignat*}{2}%
\frac{dI\_symp\_s_{3}}{dt} &= \Theta_{3}I\_{symp}\_{s}_{3} +  \mu_{3}I\_{pre}_{3} +%
\end{alignat*}%
\begin{alignat*}{2}%
\frac{dI\_symp\_m_{1}}{dt} &= \Theta_{1}I\_{symp}\_{m}_{1} +  \mu_{1}I\_{pre}_{1} +%
\end{alignat*}%
\begin{alignat*}{2}%
\frac{dI\_symp\_m_{2}}{dt} &= \Theta_{2}I\_{symp}\_{m}_{2} +  \mu_{2}I\_{pre}_{2} +%
\end{alignat*}%
\begin{alignat*}{2}%
\frac{dI\_symp\_m_{3}}{dt} &= \Theta_{3}I\_{symp}\_{m}_{3} +  \mu_{3}I\_{pre}_{3} +%
\end{alignat*}%
\begin{alignat*}{2}%
\frac{dI\_asymp_{1}}{dt} &= \Theta_{1}I\_{asymp}_{1} +  \mu_{1}I\_{pre}_{1} +%
\end{alignat*}%
\begin{alignat*}{2}%
\frac{dI\_asymp_{2}}{dt} &= \Theta_{2}I\_{asymp}_{2} +  \mu_{2}I\_{pre}_{2} +%
\end{alignat*}%
\begin{alignat*}{2}%
\frac{dI\_asymp_{3}}{dt} &= \Theta_{3}I\_{asymp}_{3} +  \mu_{3}I\_{pre}_{3} +%
\end{alignat*}%
\begin{alignat*}{2}%
\frac{dHOSP\_m_{1}}{dt} &= \Theta_{1}HOSP\_{m}_{1} +  \mu_{1}I\_{symp}\_{m}_{1} +%
\end{alignat*}%
\begin{alignat*}{2}%
\frac{dHOSP\_m_{2}}{dt} &= \Theta_{2}HOSP\_{m}_{2} +  \mu_{2}I\_{symp}\_{m}_{2} +%
\end{alignat*}%
\begin{alignat*}{2}%
\frac{dHOSP\_m_{3}}{dt} &= \Theta_{3}HOSP\_{m}_{3} +  \mu_{3}I\_{symp}\_{m}_{3} +%
\end{alignat*}%
\begin{alignat*}{2}%
\frac{dHOSP\_s_{1}}{dt} &= \Theta_{1}HOSP\_{s}_{1} +  \mu_{1}I\_{symp}\_{s}_{1} +%
\end{alignat*}%
\begin{alignat*}{2}%
\frac{dHOSP\_s_{2}}{dt} &= \Theta_{2}HOSP\_{s}_{2} +  \mu_{2}I\_{symp}\_{s}_{2} +%
\end{alignat*}%
\begin{alignat*}{2}%
\frac{dHOSP\_s_{3}}{dt} &= \Theta_{3}HOSP\_{s}_{3} +  \mu_{3}I\_{symp}\_{s}_{3} +%
\end{alignat*}%
\begin{alignat*}{2}%
\frac{dR_{1}}{dt} &= \Theta_{1}R_{1} +  \mu_{1}I\_{symp}\_{s}_{1} +  \mu_{1}I\_{symp}\_{m}_{1} +  \mu_{1}I\_{asymp}_{1} +  \mu_{1}HOSP\_{m}_{1} +  \mu_{1}HOSP\_{s}_{1} +  \\ &%
\end{alignat*}%
\begin{alignat*}{2}%
\frac{dR_{2}}{dt} &= \Theta_{2}R_{2} +  \mu_{2}I\_{symp}\_{s}_{2} +  \mu_{2}I\_{symp}\_{m}_{2} +  \mu_{2}I\_{asymp}_{2} +  \mu_{2}HOSP\_{m}_{2} +  \mu_{2}HOSP\_{s}_{2} +  \\ &%
\end{alignat*}%
\begin{alignat*}{2}%
\frac{dR_{3}}{dt} &= \Theta_{3}R_{3} +  \mu_{3}I\_{symp}\_{s}_{3} +  \mu_{3}I\_{symp}\_{m}_{3} +  \mu_{3}I\_{asymp}_{3} +  \mu_{3}HOSP\_{m}_{3} +  \mu_{3}HOSP\_{s}_{3} +  \\ &%
\end{alignat*}%
\begin{alignat*}{2}%
\frac{dS}{dt} &= \frac{R_{1}}{N} \delta_{1}\frac{R_{2}}{N} \delta_{2}\frac{R_{3}}{N} \delta_{3}-\frac{E_{1}}{N} \delta_{1}-\frac{E_{2}}{N} \delta_{2}-\frac{E_{3}}{N} \delta_{3}%
\end{alignat*}%
\end{document}